harder proofs with heq. breaks build

VCVio/OracleComp/Constructions/Replicate.lean
@@ -22,46 +22,92 @@ namespace OracleComp
 variable {ι : Type} {spec : OracleSpec ι} {α β : Type}
 
 /-- Run the computation `oa` repeatedly `n` times to get a list of `n` results. -/
-def replicate (oa : OracleComp spec α) : ℕ → OracleComp spec (List α)
-  | 0 => return []
-  | n + 1 => (· :: ·) <$> oa <*> replicate oa n
+-- def replicate (oa : OracleComp spec α) : ℕ → OracleComp spec (List α)
+--   | 0 => return []
+--   | n + 1 => (· :: ·) <$> oa <*> replicate oa n
 
 -- TODO: Decide if a version like this is better?
-def replicateᵥ (oa : OracleComp spec α) : (n : ℕ) → OracleComp spec (Vector α n)
-  | 0 => return Vector.nil
-  | n + 1 => (· ::ᵥ ·) <$> oa <*> replicateᵥ oa n
+def replicate (oa : OracleComp spec α) : (n : ℕ) → OracleComp spec (Vector α n)
+  | 0 => pure Vector.nil
+  | n + 1 => (· ::ᵥ ·) <$> oa <*> replicate oa n
+
+variable (oa : OracleComp spec α) (n m : ℕ)
 
 @[simp]
-lemma replicate_zero (oa : OracleComp spec α) : oa.replicate 0 = return [] := rfl
+lemma replicate_zero : oa.replicate 0 = pure Vector.nil := rfl
 
 @[simp]
-lemma replicate_succ (oa : OracleComp spec α) (n : ℕ) :
-    oa.replicate (n + 1) = (· :: ·) <$> oa <*> replicate oa n := rfl
+lemma replicate_succ : oa.replicate (n + 1) = (· ::ᵥ ·) <$> oa <*> replicate oa n := rfl
 
-@[simp]
+lemma replicate_add_zero : oa.replicate (n + 0) = oa.replicate n := by simp
+
+section zero_add
+
+/-- Running a computation `0 + n` times is the same as running it `n` times.
+Because `0 + n` and `n` are not definitionally equal, regular equality will not typecheck. -/
+lemma replicate_zero_add_heq : HEq (oa.replicate (0 + n)) (oa.replicate n) := by
+  cases h : 0 + n <;> {rw [zero_add] at h; cases h; rfl}
+
+/-- Running a computation `0 + n` times is the same as running it `n` times.
+Requires substituting the equality between the two to properly typecheck the vector types. -/
+lemma replicate_zero_add : oa.replicate (0 + n) = (zero_add n).symm ▸ oa.replicate n := by
+  refine eq_of_heq <| (replicate_zero_add_heq oa n).trans <| (heq_eqRec_iff_heq _ _ _).2 HEq.rfl
+
+end zero_add
+
+section comm
+
+/-- Running a computation `n + m` times is the same as running it `n` times then `m` times.
+Because `n + m` and `m + n` are not definitionally equal, regular equality will not typecheck. -/
+lemma replicate_add_comm_heq : HEq (oa.replicate (n + m)) (oa.replicate (m + n)) := by
+  cases h : n + m
+  · cases h' : m + n
+    · exact HEq.rfl
+    · rw [add_comm n m, h'] at h
+      exact (Nat.succ_ne_zero _ h).elim
+  · cases h' : m + n
+    · rw [add_comm m n, h] at h'
+      exact (Nat.succ_ne_zero _ h').elim
+    · rw [add_comm n m, h', Nat.add_one_inj] at h
+      cases h
+      rfl
+
+lemma replicate_add_comm : oa.replicate (n + m) = add_comm n m ▸ oa.replicate (m + n) := by
+  refine eq_of_heq <| (replicate_add_comm_heq oa n m).trans <| (heq_eqRec_iff_heq _ _ _).2 HEq.rfl
+
+end comm
+
+/-- Running a computation `0 + n` times is the same as running it `n` times.
+Requires substituting the equality between the two to properly typecheck the vector types. -/
 lemma replicate_add (oa : OracleComp spec α) (n m : ℕ) :
-    (replicate oa (n + m)) = (· ++ ·) <$> replicate oa n <*> replicate oa m := by
+    (replicate oa (n + m)) = Vector.append <$> replicate oa n <*> replicate oa m := by
   induction n with
-  | zero => simp only [Nat.zero_eq, zero_add, replicate_zero,
-      map_pure, List.nil_append, pure_id'_seq]
-  | succ n hn => simp only [Nat.succ_add, replicate_succ, map_eq_bind_pure_comp,
-      Function.comp, hn, seq_eq_bind, bind_assoc, pure_bind, List.cons_append]
+  | zero => {
+    refine eq_of_heq ((replicate_zero_add_heq oa m).trans ?_)
+
+    simp [seq_eq_bind, map_eq_bind_pure_comp, Function.comp]
+    sorry
+  }
+  | succ n hn => {
+    sorry
+  }
 
 lemma List.Injective2_cons {α : Type} : Function.Injective2 (List.cons (α := α)) := by
   sorry
 
 @[simp]
-lemma probOutput_replicate (oa : OracleComp spec α) (n : ℕ) (xs : List α) :
-    [= xs | replicate oa n] = if xs.length = n then (xs.map ([= · | oa])).prod else 0 := by
-  match xs with
-  | [] => sorry
-  | x :: xs => {
-    induction n with
-    | zero => sorry
-    | succ n hn => {
-      sorry
-    }
-  }
+lemma probOutput_replicate (oa : OracleComp spec α) (n : ℕ) (xs : Vector α n) :
+    [= xs | replicate oa n] = (xs.toList.map ([= · | oa])).prod := by
+  sorry
+  -- match xs with
+  -- | [] => sorry
+  -- | x :: xs => {
+  --   induction n with
+  --   | zero => sorry
+  --   | succ n hn => {
+  --     sorry
+  --   }
+  -- }
   -- induction n with
   -- | zero => cases xs <;> simp
   -- | succ n hn => {
@@ -76,9 +122,11 @@ lemma probOutput_replicate (oa : OracleComp spec α) (n : ℕ) (xs : List α) :
   --   }
   -- }
 
+#check Vector
+
 @[simp]
 lemma support_replicate (oa : OracleComp spec α) (n : ℕ) :
-    (replicate oa n).support = {xs | ∀ x ∈ xs, x ∈ oa.support} := by
+    (replicate oa n).support = {xs | ∀ x ∈ xs.toList, x ∈ oa.support} := by
   sorry
 
 /-- Vectors can be selected uniformly if the underlying type can be.
